git-svn-id: https://scm.gforge.inria.fr/svn/easycrypt/branches/modules@2758 4a0602ed-0ddf-4d1e-8465-5e6d797b7344

theories/Set.ec
@@ -1,6 +1,8 @@
 require import int.
 require import Fun.
 
+ prover 1 10 "Alt-Ergo" "Vampire" "Z3" "CVC3".
+
 type 'a t.
 
 cnst empty : 'a t.
@@ -9,70 +11,377 @@ op add    : ('a, 'a t) -> 'a t.
 
 op singleton (x:'a) : 'a t = add x empty.
 
+op pick   : 'a t -> 'a.
 op rm     : ('a, 'a t) -> 'a t.
 op union  : ('a t, 'a t) -> 'a t.
 op inter  : ('a t, 'a t) -> 'a t.
 
 op is_empty : 'a t -> bool.
+axiom is_empty_empty : forall (X : 'a t), is_empty X <=> X = empty.
+
 
 op mem      : ('a, 'a t) -> bool.
 op Pmem (X:'a t, x:'a) : bool = mem x X.
 
-op card     : 'a t -> int.
+axiom Set_ind : forall (P : ('a t) Pred),
+P empty =>
+(forall (S : 'a t, x : 'a), !mem x S => P S => P (add x S)) =>
+ forall (S : 'a t), P S.
 
-axiom card_pos : forall (X:'a t), 0 <= card X. 
+op card     : 'a t -> int.
+axiom card1 : card<:'a> empty = 0.
+axiom cadr2 : forall (S : 'a t, x : 'a), mem x S => card(S) = 1 + card(rm x S).
 
 pred [==] (X1:'a t, X2:'a t) = 
-  forall (x:'a), mem x X1 <=> mem x X2.
+ forall (x:'a), mem x X1 <=> mem x X2.
+
+ (* extentional equality is an equivalence relation*)
+lemma eq_refl :
+ forall (X:'a t), X == X.
+
+lemma eq_sym :
+ forall (X Y:'a t), X == Y => Y == X.
+
+
+lemma eq_trans :
+ forall (X Y Z:'a t), X == Y => Y == Z => X == Z.
+
+
+pred [<=] (X1:'a t, X2:'a t) = 
+ forall (x:'a), mem x X1 => mem x X2.
+
+ (* subset defines a Poset *)
+lemma sub_refl :
+ forall (X:'a t), X <= X.
+
+lemma sub_anti_sym : 
+ forall (X Y:'a t), X <= Y => Y <= X => X == Y.
+
+lemma sub_trans :
+ forall (X Y Z:'a t), X <= Y => Y <= Z => X <= Z.
 
 axiom extentionnality : 
-  forall (X1:'a t, X2:'a t),
-     X1 = X2 <=> X1 == X2.
+ forall (X1:'a t, X2:'a t),
+X1 = X2 <=> X1 == X2.
 
-(* Specification of is_empty *)
+
+ (* Specification of is_empty *)
 axiom is_empty_mem : forall (X:'a t), 
-   is_empty X <=> forall (x:'a), !mem x X.
+ is_empty X <=> forall (x:'a), !mem x X.
 
-axiom is_empty_card : forall (X:'a t),
-   is_empty X <=> card X = 0.
+ (* local *) pred P_is_empty_card (X : 'a t) =
+card X = 0 => is_empty X.
 
-(* Specification of empty *)
-axiom is_empty_empty : is_empty<:'a> empty<:'a>.
+ (* Specification of empty *)
 
-(* FIXME lemma *)
-axiom empty_mem  : forall (x:'a), !mem x empty.
+lemma empty_subset : forall(X:'a t),
+ empty <= X.
+
+ (* FIXME lemma *)
+lemma empty_mem  : forall (x:'a), !mem x empty.
 
 axiom empty_card : card<:'a>(empty) = 0.
 
-(* Specification of add *)
+ (* Specification of add *)
 
 axiom add_mem : forall (x:'a, y:'a, X:'a t), 
-   mem x (add y X) <=> mem x X || x = y.
+ mem x (add y X) <=> mem x X || x = y.
+
 
 axiom add_card : forall (x:'a, X:'a t), 
-   !mem x X => card (add x X) = card X + 1.
+ !mem x X => card (add x X) = card X + 1.
 
-(* Need to put extentionality, to get it as a lemma *)
-axiom mem_add : forall (x:'a, X:'a t),
-   mem x X => X = add x X.
+lemma mem_add_aux : forall (x:'a, X:'a t),
+mem x X => X == add x X.
 
-axiom singleton_card : forall (x:'a),
-   card (singleton x) = 1.
+lemma mem_add : forall (x:'a, X:'a t),
+mem x X => X = add x X.
 
-(* filter *)
+lemma add_subset : forall  (x:'a, X:'a t),
+ X <= add x X.
+
+lemma singleton_card : forall (x:'a),
+card (singleton x) = 1.
+
+ (* local *) pred P_card_pos (X : 'a t) = 0 <= card X.
+lemma card_pos : forall (X:'a t), 0 <= card X
+proof.
+ intros X.
+ cut H : (P_card_pos X).
+ apply Set_ind<:'a>(P_card_pos,_,_,X);trivial.
+ trivial.
+save.
+
+
+  (* filter *)
 op filter : ('a Pred, 'a t) -> 'a t.
 
 axiom filter_mem : forall (P:'a Pred, X:'a t, x:'a),
-   mem x (filter P X) <=> (mem x X && P x).
+ mem x (filter P X) <=> (mem x X && P x).
 
 axiom filter_card : forall (P:'a Pred, X : 'a t), 
-   card (filter P X) = card X - card(filter (Pnot P) X). 
+card (filter P X) = card X - card(filter (Pnot P) X). 
 
 axiom filter_Peq_in : forall (x:'a, X:'a t),
-   mem x X =>
-   filter (Peq x) X = singleton x.
+mem x X =>
+filter (Peq x) X = singleton x.
 
 axiom filter_Peq_card_in : forall (x:'a, X:'a t),
-   mem x X =>
-   card (filter (Peq x) X) = 1.
-     
+mem x X =>
+card (filter (Peq x) X) = 1.
+
+lemma filter_subset : forall (P:'a Pred, X:'a t),
+ filter P X <= X.
+
+ (* facts about pick *)
+axiom pick_spec : forall (X : 'a t), 
+ X <> empty => mem (pick X) X.
+
+lemma pick_singleton : forall (x : 'a), 
+pick (singleton x) = x.
+
+ (* facts about rm *)
+axiom rm_spec_not_mem : forall(X :'a t, x: 'a),
+ !mem x X => rm x X = X.
+
+axiom rm_spec_mem : forall(X :'a t, x: 'a),
+mem x X => add x (rm x X) = X.
+
+axiom rm_mem : forall (X : 'a t, x : 'a),
+ !mem x (rm x X).
+
+lemma rm_subs :  forall (X : 'a t, x : 'a),
+ rm x X <= X.
+
+lemma rm_card :  forall (X : 'a t, x : 'a),
+ card(rm x X) <= card X.
+
+lemma card_non_empty : forall (X : 'a t),
+ forall (x :'a),
+mem x X => card<:'a> X = 1 + card (rm x X).
+
+lemma is_empty_card : forall (X:'a t),
+card X = 0 => is_empty X 
+proof.
+ intros X.
+ cut H : (P_is_empty_card X).
+ apply Set_ind<:'a>(P_is_empty_card,_,_,X);trivial.
+ trivial.
+save.
+
+  (* union *) 
+axiom union_mem : forall(X:'a t, Y:'a t, x: 'a),
+ mem x (union X Y) <=> (mem x X || mem x Y).
+
+lemma union_empty : forall(X :'a t),
+union X empty = X
+proof.
+ intros X.
+ cut H : (union X empty == X).
+ trivial.
+ trivial.
+save.
+
+lemma union_empty_aux : forall(X :'a t),
+union X empty == X.
+
+
+lemma union_comm1 : forall(X:'a t, Y:'a t),
+union X Y == union Y X.
+
+lemma union_comm : forall(X:'a t, Y:'a t),
+union X Y = union Y X.
+
+lemma union_add_aux : forall(X:'a t, Y:'a t, x: 'a),
+add x (union X Y) == union (add x X) Y.
+
+lemma union_add : forall(X:'a t, Y:'a t, x: 'a),
+add x (union X Y) = union (add x X) Y.
+
+lemma subset_union1 : forall (X Y : 'a t),
+ X <= union X Y.
+
+ (* local *) pred P_subset_union (X : 'a t) = forall(Y : 'a t),
+ X <= Y => exists (Z : 'a t), Y = union X Z.
+
+lemma subset_union2 : forall (X : 'a t, Y : 'a t),
+ X <= Y => exists (Z : 'a t), Y = union X Z
+proof.
+ intros X.
+ cut H0 : (P_subset_union X).
+ apply Set_ind<:'a>(P_subset_union,_,_,X).
+ trivial.
+ intros S x H H0.
+ cut H1 : (forall (Y : 'a t), (add x S)<= Y => (exists (Z : 'a t), Y = union (add x S) Z)).
+ intros Y H1.
+ cut H2 : (S <= Y).
+ trivial.
+ cut H3 : (forall(Y : 'a t),
+ S <= Y => exists (Z : 'a t), Y = union S Z).
+ trivial.
+ cut H4 : (exists (Z : 'a t), Y = union S Z).
+ apply H3(Y,_).
+ assumption.
+ elim H4.
+ intros Z H5.
+ trivial.
+ trivial.
+ trivial.
+save.
+
+
+  (* local *) pred P_union_card1( X : 'a t) = forall(Y :'a t),
+  card (union X Y) <= card(X) + card(Y).
+
+lemma union_card1 : forall (X:'a t, Y:'a t),
+ card (union X Y) <= card (X) + card(Y)
+proof.
+ intros X.
+ cut H : (P_union_card1 X).
+ apply Set_ind<:'a>(P_union_card1,_,_,X);trivial.
+ trivial.
+save.
+
+pred P_union_card2( Y : 'a t) = forall(X:'a t),
+ card X <= card (union X Y).
+
+lemma union_card2 : forall (Y:'a t, X:'a t),
+ card X <= card (union X Y)
+proof. 
+ intros Y.
+ cut H : (P_union_card2 Y).
+ apply Set_ind<:'a>(P_union_card2,_,_,Y). 
+ trivial.
+ intros S x H H1.
+ cut H0 : (forall(X:'a t),
+ card X <= card (union X (add x S))).
+ intros X.
+ cut H2: (card X <= card (union X S)).
+ trivial.
+ cut H3: (card (union X S) <= card (union X (add x S))).
+ cut H4: (card (union X (add x S)) = card (add x (union X S))).
+ trivial.
+ trivial.
+ trivial.
+ trivial.
+ trivial.
+save.
+
+
+  (* subset card *)
+
+lemma susbset_card : forall (Y : 'a t, X : 'a t),
+ X <= Y => (card X) <= (card Y)
+proof.
+ intros Y X H.
+ cut H0: (exists (Z : 'a t), Y = union X Z).
+ trivial.
+ elim H0.
+ intros Z H1.
+ cut H2: (card X <= card (union X Z)).
+ trivial.
+ trivial.
+save.
+
+  (* intersection *)
+axiom inter_mem : forall(X:'a t, Y:'a t, x: 'a),
+ mem x (inter X Y) <=> (mem x X && mem x Y).
+
+lemma inter_empty : forall(X :'a t),
+inter X empty = empty
+proof.
+ intros X.
+ cut H : (inter X empty == empty).
+ trivial.
+ trivial.
+save.
+
+lemma inter_comm : forall(X:'a t, Y:'a t),
+inter X Y = inter Y X 
+proof.
+ intros X Y.
+ cut H: (inter X Y == inter Y X).
+ trivial.
+ trivial.
+save.
+
+lemma inter_add : forall(X:'a t, Y:'a t, x: 'a),
+add x (inter X Y) = inter (add x X) (add x Y)
+proof.
+ intros X Y x.
+ cut H: (add x (inter X Y) == inter (add x X) (add x Y)).
+ trivial.
+ trivial.
+save.
+
+lemma inter_add2 :forall(X : 'a t, Y : 'a t, x : 'a),
+mem x Y =>
+add x (inter X Y) = inter (add x X)  Y
+proof.
+ intros X Y x H.
+ cut H0: (add x (inter X Y) == inter (add x X)  Y).
+ trivial.
+ trivial.
+save.
+
+
+lemma inter_add3 :forall(X : 'a t, Y : 'a t, x : 'a),
+ !mem x Y =>
+(inter X Y) = inter (add x X)  Y
+proof.
+ intros X Y x H.
+ cut H0: ((inter X Y) == inter (add x X)  Y).
+ trivial.
+ trivial.
+save.
+
+lemma subset_inter : forall (X Y : 'a t),
+ inter X Y <= X.
+
+lemma card_inter : forall (X Y : 'a t),
+ card (inter X Y) <= card X.
+
+pred P_union_inter(X: 'a t) = forall(Y : 'a t),
+ card(union X Y) + card(inter X Y) = card(X) + card(Y).
+
+lemma card_union_inter : forall (X Y: 'a t),
+ card(union X Y) + card(inter X Y) = card(X) + card(Y)
+proof. 
+ intros X.
+ cut H: (P_union_inter X).
+ apply Set_ind<:'a>(P_union_inter,_,_, X).
+ trivial.
+ intros S x H H0.
+ cut H1 : (forall (Y : 'a t),
+ card(union (add x S) Y) + card(inter (add  x S) Y) = card(add x S) + card(Y)).
+ intros Y.
+ cut H8: (card(union S Y) + card(inter S Y) = card(S) + card(Y)).
+ trivial.
+ cut H2 : (mem x Y =>
+ card(union (add x S) Y) + card(inter (add  x S) Y) = card(add x S) + card(Y)).
+ intros H3.
+ cut H4: (card (add x (inter S Y)) = card(inter (add x S) Y)).
+ cut H5: (add x (inter S Y) = (inter (add x S) Y)).
+ trivial.
+ trivial.
+ cut H5: (!mem x (inter S Y)).
+ trivial.
+ cut H6 : (card(inter (add  x S) Y) = 1 + card (inter S Y)).
+ trivial.
+ cut H7: (card(add x S) = 1 + card S).
+ trivial.
+ trivial.
+ cut H3 : (!mem x Y =>
+ card(union (add x S) Y) + card(inter (add  x S) Y) = card(add x S) + card(Y)).
+ intros H4.
+ cut H5: (card (inter S Y) = card(inter (add x S) Y)).
+ trivial.
+ cut H6: (!mem x (union S Y)).
+ trivial.
+ cut H7: (card(union(add x S) Y) = 1 + card(union S Y)).
+ trivial.
+ trivial.
+ trivial.
+ trivial.
+ trivial.
+save.
